naming changes. bundles added, need 2 check matches defs

strands.v
@@ -17,13 +17,13 @@
    http://www.mitre.org/work/tech_papers/tech_papers_01/guttman_bundles/
  *)
 
-Require Import List Arith Peano_dec Omega Ensembles.
+Require Import List Arith Peano_dec Omega Ensembles Finite_sets.
 
 (* Represent atomic messages, *)
-Variable text : Set.
+Variable Text : Set.
 
 (* representing kryptographic key *)
-Variable key : Set.
+Variable Key : Set.
 (* TODO - injective, unary operation (inv : key -> key)
           Or in Coq would this make more sense
           instead as  key -> key -> Prop?
@@ -36,40 +36,40 @@ Variable key : Set.
    associated with a specific name.*)
 
 (* message or term *)
-Inductive msg : Type :=
-| mtext : text -> msg
-| mcons : msg -> msg -> msg 
-| mcrypt : key -> msg -> msg.
+Inductive Msg : Type :=
+| msg_text : Text -> Msg
+| msg_app : Msg -> Msg -> Msg 
+| msg_crypt : Key -> Msg -> Msg.
 (* [REF 1] Section 2.1 pg 5 
            Section 2.3 pg 9 *)
 (* [REF 2] pg 4 paragraph 3 (detains of encryption and subterms) *)
-Hint Constructors msg.
+Hint Constructors Msg.
 
 (* subterm relationship for messages *)
 (* subterm -> larger encapsulating term -> Prop *)
-Inductive subterm : msg -> msg -> Prop :=
-| strefl : forall m, subterm m m
+Inductive Subterm : Msg -> Msg -> Prop :=
+| st_refl : forall m, Subterm m m
 (* | stcryp : forall a g, subterm a g -> subterm a encrpt(g)  *)
-| stcons_l : forall st l r, 
-               subterm st l -> subterm st (mcons l r)
-| stcons_r : forall st l r, 
-               subterm st r -> subterm st (mcons l r)
-| stcrpyt : forall st t k, 
-              subterm st t -> subterm st (mcrypt k t).
+| st_app_l : forall st l r, 
+               Subterm st l -> Subterm st (msg_app l r)
+| st_app_r : forall st l r, 
+               Subterm st r -> Subterm st (msg_app l r)
+| st_crpyt : forall st t k, 
+              Subterm st t -> Subterm st (msg_crypt k t).
 (* [REF 1] Definition 2.1 pg 6 and Definition 2.11 *)
-Hint Constructors subterm.
+Hint Constructors Subterm.
 
 (* signed message, + (tx) or - (rx) *)
-Inductive smsg : Type := 
-| tx : msg -> smsg
-| rx : msg -> smsg.
+Inductive SMsg : Type := 
+| tx : Msg -> SMsg
+| rx : Msg -> SMsg.
 (* [REF 1] Definition 2.1 pg 6 
    They are defined as a pair, w/ the first member being in {+, -} 
    and the second a signed message. *)
-Hint Constructors smsg.
+Hint Constructors SMsg.
 
 (* strand *)
-Definition strand : Type := list smsg.
+Definition Strand : Type := list SMsg.
 (* [REF 1] First sentence of Abstract: "sequence of events"  
    Haven't hit a better def, and they start using strands
    pretty early so I'm rolling with this. *)
@@ -78,51 +78,59 @@ Definition strand : Type := list smsg.
 Definition strand_in_set (s:strand) (ss:set strand) : bool := 
   set_mem strand_eq_dec s ss. *)
 
-(* strand space *)
-Inductive sspace : Type :=
-| space : Ensemble msg -> Ensemble strand -> sspace.
-(* [REF 1] Definition 2.2 pg 6 "A strand space over A (set of possible msgs) 
-           is a set E with a trace mapping tr : E -> list smsg *)
+Definition Strands := Ensemble Strand.
+Definition Msgs := Ensemble Msg.
+Definition SMsgs := Ensemble SMsg.
 
-Definition ss_msgs (ss:sspace) : Ensemble msg :=
+(* strand space *)
+Inductive StrandSpace : Type :=
+| strandspace : Msgs -> Strands -> StrandSpace.
+(* [REF 1] Definition 2.2 pg 6 "A strand space over A (set of possible msgs) 
+           is a set E with a trace mapping tr : E -> list smsg" *)
+
+Definition SS_msgs (ss:StrandSpace) : Msgs :=
  match ss with
-  | space m_set s_set => m_set
+  | strandspace m_set s_set => m_set
  end.
 
-Definition ss_strands (ss:sspace) : Ensemble strand :=
+Definition SS_strands (ss:StrandSpace) : Strands :=
  match ss with
-  | space m_set s_set => s_set
+  | strandspace m_set s_set => s_set
  end.
 
 
 (* node in a strand space *)
-Definition node : Type := {n: (prod strand nat) | (snd n) < (length (fst n))}.
+Definition Node : Type := {n: (prod Strand nat) | (snd n) < (length (fst n))}.
 (* [REF 1] Definition 2.3.1 pg 6
    -"A node is a pair <s,i> where s is a strand and i a nat in [0, (length s))"
      NOTE: I changed it to be 0 based instead of 1 based sequences
    -"node <s,i> belongs to strand s"
    -"Every node belongs to a unique strand" *)
 
+Definition Edge : Type := (prod Node Node).
+Definition Nodes := Ensemble Node.
+Definition Edges := Ensemble Edge.
+
 (* index of a node *)
-Definition n_index (n:node) : nat :=
+Definition Node_index (n:Node) : nat :=
   match n with
     | exist npair _ 
       => snd npair
   end.
 (* [REF 1] Definition 2.3.2 pg 6
-   "If n = <s,i> then index(n) = i. *)
+   "If n = <s,i> then index(n) = i." *)
 
 (* strand of a node *)
-Definition n_strand (n:node) : strand :=
+Definition Node_strand (n:Node) : Strand :=
   match n with
     | exist npair _ 
       => fst npair
   end.
 (* [REF 1] Definition 2.3.2 pg 6
-   "If n = <s,i> then ... strand(n) = s. *)
+   "If n = <s,i> then ... strand(n) = s." *)
 
 (* signed message of a node *)
-Fixpoint n_smsg_option (n:node) : (option smsg) :=
+Fixpoint Node_smsg_option (n:Node) : (option SMsg) :=
   match n with
     | exist (s, i) p 
       =>  nth_error s i
@@ -150,30 +158,30 @@ Proof.
   simpl. omega. 
 Qed.
 
-Theorem n_smsg_valid : forall (n:node),
-{m:smsg | Some m = n_smsg_option n}.
+Theorem Node_smsg_valid : forall (n:Node),
+{m:SMsg | Some m = Node_smsg_option n}.
 (* exists (m:smsg), Some m = (n_smsg_option n). *)
 Proof.
   intros n.
-  remember (n_smsg_option n) as funcall.
+  remember (Node_smsg_option n) as funcall.
   destruct n. destruct funcall.  
   exists s. reflexivity.
 
-  unfold n_smsg_option in Heqfuncall.
+  unfold Node_smsg_option in Heqfuncall.
   destruct x. simpl in l.
   apply nth_error_len in Heqfuncall.
   omega.
 Qed.
 
 (* signed message of a node *)
-Definition n_smsg (n:node) : smsg :=
- match n_smsg_valid n with
+Definition Node_smsg (n:Node) : SMsg :=
+ match Node_smsg_valid n with
      | exist m _ => m
  end.
 
 (* unsigned message of a node *)
-Fixpoint n_msg (n:node) : msg :=
-  match n_smsg n with
+Fixpoint Node_msg (n:Node) : Msg :=
+  match Node_smsg n with
     | tx t => t
     | rx t => t
   end. 
@@ -182,79 +190,141 @@ Fixpoint n_msg (n:node) : msg :=
     of the trace of s." *)
 
 (* To reason about the set of nodes in a strand space *)
-Definition node_in_ss (n:node) (ss:sspace) : Prop := 
- In strand (ss_strands ss) (n_strand n).
+Definition NodeInSS (n:Node) (ss:StrandSpace) : Prop := 
+ In Strand (SS_strands ss) (Node_strand n).
 (* [REF 1] Definition 2.3.1 pg 6
    The reference to the "set of nodes (N) in a given strand space." *)
 
 (* Set of all nodes in a strand space *)
-Definition nodeset (ss:sspace) : Type := 
-{ns: Ensemble node | forall n, (node_in_ss n ss)  <-> In node ns n}.
+Definition NodeSet (ss:StrandSpace) : Type := 
+{ns: Nodes | forall n, (NodeInSS n ss)  <-> In Node ns n}.
 (* [REF 1] Definition 2.3.1 pg 6
    The set of nodes (in a strand space) is denoted by N. *)
 
-Inductive comm_E : node -> node -> Prop :=
-| commE :  forall n m, (exists a, (and ((n_smsg n) = (tx a)) 
-                                 ((n_smsg m) = (rx a))))
-                             -> comm_E n m.
+Inductive CommEdge : Node -> Node -> Prop :=
+| c_edge :  forall n m, (exists a, (and ((Node_smsg n) = (tx a)) 
+                                 ((Node_smsg m) = (rx a))))
+                             -> CommEdge n m.
 (* [REF 1] Definition 2.3.3 pg 6
    "there is an edge n1 -> n2 iff term(n1) = +a and term(n2) = -a." *)
 
 (* predecessor edge *)
 (* node's direct predecessor -> node -> Prop *)
-Inductive pred_E : node -> node -> Prop :=
-| predE : forall i j, n_strand i = n_strand j 
-                      -> (n_index i) + 1 = (n_index j) 
-                      -> pred_E i j.
+Inductive PredEdge : Node -> Node -> Prop :=
+| p_edge : forall i j, Node_strand i = Node_strand j 
+                      -> (Node_index i) + 1 = (Node_index j) 
+                      -> PredEdge i j.
 (* [REF 1] Definition 2.3.4 pg 6
    "When n1= <s,i> and n2=<s,i+1> are members of N (set of node), there is
     an edge n1 => n2." *)
 
 (* predecessor multi edge (not nec. immediate predecessor) *)
 (* node's predecessor -> node -> Prop *)
-Inductive predX_E : node -> node -> Prop :=
-| predXE1 : forall i j, pred_E i j -> predX_E i j
-| predXEX : forall i j k, pred_E i j -> predX_E j k -> predX_E i k.
+Inductive PredPath : Node -> Node -> Prop :=
+| ppath_step : forall i j, PredEdge i j -> PredPath i j
+| ppath_path : forall i j k, PredEdge i j -> PredPath j k -> PredPath i k.
 (* [REF 1] Definition 2.3.4 pg 6
    "ni =>+ nj means that ni precedes nj (not necessarily immediately) on
     the same strand." *)
 
-Inductive occurs_in : msg -> node -> Prop :=
-| occursin : forall m n, subterm m (n_msg n) -> occurs_in m n.
+(* A Path (traversing either edge Types) of length
+   1 or more. *)
+Inductive FwdPath : Node -> Node -> Prop :=
+| path_comm : forall x y, CommEdge x y -> FwdPath x y
+| path_pred : forall x y, PredPath x y -> FwdPath x y
+| path_comm_path : forall x y z, CommEdge x y -> FwdPath y z -> FwdPath x z
+| path_pred_path : forall x y z, PredPath x y -> FwdPath y z -> FwdPath x z.
+
+Inductive OccursIn : Msg -> Node -> Prop :=
+| occurs_in : forall m n, Subterm m (Node_msg n) -> OccursIn m n.
 (* [REF 1] Definition 2.3.5 pg  6
    "An unsigned term m occurs in a node n iff m is a subterm of term(n). " *)
 
 (* signifies the origin of a msg. *)
-Inductive entry_point : node -> Ensemble msg -> Prop :=
+Inductive EntryPoint : Node -> Msgs -> Prop :=
  | entrypoint :  forall n I, 
-    (and (exists m, (and ((n_smsg n) = (tx m)) 
-                         (In msg I m)))
-         (forall n', (predX_E n' n) 
-                     -> ~(In msg I (n_msg n'))))
-    -> entry_point n I.
+    (and (exists m, (and ((Node_smsg n) = (tx m)) 
+                         (In Msg I m)))
+         (forall n', (PredPath n' n) 
+                     -> ~(In Msg I (Node_msg n'))))
+    -> EntryPoint n I.
 (* [REF 1] Definition 2.3.6 pg 6
    "The node n in N is an entry point for I (a set of unsigned terms) iff
     term(n) = +t for some t in I, and whenever n' =>+ n term(n') is not in I."*)
 
 (* where an unsigned term originates, what node *)
-Inductive orig_at : msg -> node -> Prop :=
-| origat : forall m n, 
-             (exists I, (and (entry_point n I)
-                             (forall m', In msg I m -> subterm m m')))
-             -> orig_at m n.
+Inductive OriginateAt : Msg -> Node -> Prop :=
+| orig_at : forall m n, 
+             (exists I, (and (EntryPoint n I)
+                             (forall m', In Msg I m -> Subterm m m')))
+             -> OriginateAt m n.
 (* [REF 1] Definition 2.3.7 pg 6
    "An unsigned term t originates on n in N iff n is an entry point for 
     the set I = {t' | t is a subterm of t'}."*)
 
 (* uniquely originating term def, useful for nonces or session keys *)
-Inductive uniq_orig : msg -> Prop :=
-| uniqorg : forall t, (exists n, 
-              (forall n', orig_at t n' -> n = n') )
-              -> uniq_orig t.
+Inductive UniqOrigin : Msg -> Prop :=
+| uniq_orig : forall t, (exists n, 
+              (forall n', OriginateAt t n' -> n = n') )
+              -> UniqOrigin t.
 (* [REF 1] Definition 2.3.8 pg 7 
    "unsigned term t is uniquely originating iff t originates on a unique
     n in N." *)
 
+Inductive InP (X:Type) : Ensemble (X*X) -> X -> Prop :=
+| inp_l : forall E x,
+           (exists y, In (X*X) E (x,y))
+           -> InP X E x
+| inp_r : forall E x,
+           (exists y, In (X*X) E (y,x))
+           -> InP X E x.
+
+Inductive ValidNodes : Nodes -> Prop :=
+| vn : forall N, Finite Node N -> ValidNodes N.
+
+Inductive ValidEdges : Nodes -> Edges -> Prop :=
+| ve : forall N E,
+         (and (Finite Edge E) 
+              (forall n, InP Node E n -> In Node N n)) ->
+         ValidEdges N E.
+
+Inductive Acyclic : Nodes -> Prop :=
+| acyclic : forall N,
+ (forall n, (and (In Node N n) 
+                (~ FwdPath n n))) -> Acyclic N.
 
 (* Definition bundle : *)
-(* [REF 1] Definition 2.4 pg 7 *)
+
+Definition EdgesWitness N2 P :=
+ (forall n m, In (Node*Node) N2 (n,m) -> P n m).
+
+(* *)
+Inductive Bundle : Nodes -> Edges -> Edges -> Prop :=
+| ssbundle : forall (N:Nodes) (CE PE:Edges),
+               Finite Node N -> 
+               Finite Edge CE -> 
+               Finite Edge PE ->
+               ValidEdges N CE ->
+               ValidEdges N PE ->
+               EdgesWitness CE CommEdge ->
+               EdgesWitness PE PredEdge ->
+               Acyclic N -> 
+               Bundle N CE PE.
+(* [REF 1] Definition 2.4 pg 7 
+    1) The subgraph is finite
+    2) If n2 is in Nodes and is a rx-ing message, then there
+       is a unique n1 in CE such that n1 transmist that message
+       to n2
+    3) If n2 is in Nodes and PredEdge n1 n2 then that edge
+       is in PE.
+    4) The subgraph is acyclic 
+    
+    -Additionally
+     - A strand may send or tx or rx a msg, but not 
+       both simultaneously (given by def of SMsg)
+     - When a strand rx a msg, there is a unique node 
+       tx that msg
+     - when a strand transmits a msg, many strands may
+       immediately rx that msg
+*)
+ 
